LemmasForClauses.AndClauses.fst
@@ -49,9 +49,9 @@ let and_clauses_in_interval (v1:int) (v2:int) (v:int) (n:nat) (start_interval:na
 
 #set-options "--split_queries always"
 let prove_same_value_can_extend_and (f1:formula_t) (rf1 : list (list int)) (v1:int)
-                         (f2:formula_t) (rf2 : list (list int)) (v2:int)
-                         (n:nat) (start_interval:nat) (mid:nat) (v:int) (end_interval:nat)
-                         (rf : list (list int))
+                                    (f2:formula_t) (rf2 : list (list int)) (v2:int)
+                                    (n:nat) (start_interval:nat) (mid:nat) (v:int) (end_interval:nat)
+                                    (rf : list (list int))
     : Lemma (requires n <= start_interval /\ start_interval <= mid /\ mid <= v /\
                       valid f1 rf1 v1 n start_interval mid /\
                       tseitin_same_value f1 rf1 v1 n start_interval mid /\
