Main.fst
@@ -38,16 +38,7 @@ let main = let f0 = Var 0 in
            let f2 = Var 2 in
            let f3 = Var 3 in 
 
-           let var_for_rule_0 = DImplies f0 f1 in
-           let var_for_rule_1 = Implies f0 f1 in
-           let var_for_rule_2 = Or f0 (And f1 f2) in
-           let var_for_rule_3 = Or (And f1 f2) (DImplies f0 f1) in
-           let var_for_rule_5 = Or f0 (Or f1 f2) in
-           let var_for_rule_6 = And f0 (And f1 f2) in
-           let var_for_rule_7 = Not (And f0 f1) in
-           let var_for_rule_8 = Not (Or f0 f1) in
-           let var_for_rule_9 = Not (Not f0) in
-           let test_formula = DImplies (Or f1 f2) f0 in
+           let test_formula = Or (And f1 f2) (Not (Or (DImplies f0 f1) f3)) in
 
            let out1 = FStar.Printf.sprintf "Formula: %s\n\n" (pretty_print test_formula) in
            print_string out1;
